pulse/src/checker/Pulse.ElimGoto.fst
@@ -230,8 +230,8 @@ let rec conditionalize (g: env) (t: st_term) (cond: cond_params) : T.Tac (option
     else
       None
   | Tm_While { invariant; condition; condition_var; body } -> 
-    conditionalize g { t with term = Tm_NuWhile { invariant; condition; body } } cond
-  | Tm_NuWhile { invariant; condition; body } -> (
+    conditionalize g { t with term = Tm_NuWhile { invariant; condition; cont_req = tm_unknown; body } } cond
+  | Tm_NuWhile { invariant; cont_req; condition; body } -> (
     let x = fresh g in
     let cond_cond = { cond with result = Some { n = ppname_default; x; ty = tm_bool } } in
     let cond_body = { cond with result = None } in
@@ -241,6 +241,7 @@ let rec conditionalize (g: env) (t: st_term) (cond: cond_params) : T.Tac (option
       let y = fresh g in
       Some { t with term = Tm_NuWhile {
         invariant;
+        cont_req;
         condition = wtag condition.effect_tag <|
           Tm_Bind {
             head = mk_read u0 tm_bool (term_of_nvar cond.cond);
@@ -359,9 +360,10 @@ let rec elim_gotos (g: env) (t: st_term) : T.Tac st_term =
       condition_var;
       body = elim_gotos g body;
     } }
-  | Tm_NuWhile { invariant; condition; body } ->
+  | Tm_NuWhile { invariant; cont_req; condition; body } ->
     { t with term = Tm_NuWhile {
       invariant;
+      cont_req;
       condition = elim_gotos g condition;
       body = elim_gotos g body;
     } }
