pulse/src/checker/Pulse.Typing.fst
@@ -1019,6 +1019,7 @@ type st_typing : env -> st_term -> comp -> Type =
       st_typing g cond (comp_nuwhile_cond inv post_cond) ->
       st_typing g body (comp_nuwhile_body inv post_cond) ->
       st_typing g (wtag (Some STT) (Tm_NuWhile { invariant = inv;
+                                               cont_req = tm_unknown;
                                                condition = cond;
                                                body }))
                   (comp_nuwhile inv post_cond)
