pulse/src/syntax_extension/PulseSyntaxExtension.Sugar.fst
@@ -111,6 +111,7 @@ type while_invariant1 =
   | Old of ident & slprop
   | New of slprop
   | BreakRequires of A.term
+  | ContinueRequires of A.term
 
 type while_invariant = list while_invariant1
 
@@ -286,6 +287,7 @@ instance showable_while_invariant1 : showable while_invariant1 = {
     | Old x -> "Old " ^ show x
     | New x -> "New " ^ show x
     | BreakRequires x -> "BreakRequires " ^ show x
+    | ContinueRequires x -> "ContinueRequires " ^ show x
     );
 }
 
@@ -386,6 +388,7 @@ let eq_while_invariant1 (i1 i2:while_invariant1) =
   | Old (id1, t1), Old (id2, t2) -> eq_ident id1 id2 && eq_slprop t1 t2
   | New t1, New t2 -> eq_slprop t1 t2
   | BreakRequires t1, BreakRequires t2 -> AD.eq_term t1 t2
+  | ContinueRequires t1, ContinueRequires t2 -> AD.eq_term t1 t2
   | _, _ -> false
 
 let rec eq_decl (d1 d2:decl) =
@@ -572,6 +575,7 @@ and scan_while_invariant1 (cbs:A.dep_scan_callbacks) (i:while_invariant1) =
   | Old (id, t) -> cbs.scan_term t
   | New t -> cbs.scan_term t
   | BreakRequires t -> cbs.scan_term t
+  | ContinueRequires t -> cbs.scan_term t
 and scan_stmt (cbs:A.dep_scan_callbacks) (s:stmt) =
   match s.s with
   | Open l -> cbs.add_open l
